Kraken/X64/Semantics.lean
@@ -408,7 +408,7 @@ def CondCode.interp (cc : CondCode) (s : StatusFlags) : Bool := match cc with
 @[kstep] def ShiftCountExpr.interpMasked [Labels] (c : ShiftCountExpr) (s : MachineData) (p : Std.Rco Int64) (w : Width) : Nat :=
   (c.interp s p).toNat &&& match w with | .W64 => 0x3f | _ => 0x1f -- "masked to 5 bits (or 6 bits with a 64-bit operand)"
 
-def RelRegOrMem.interp [Labels] [AddressSize]
+@[kstep] def RelRegOrMem.interp [Labels] [AddressSize]
   (o : RelRegOrMem) (s : MachineData) (p : Std.Rco Int64)
   (ret : BitVec 64 → MachineData → Effects) :=
   match o with
